formal/pickles/Pickles/StepProof.lean
@@ -238,7 +238,7 @@ theorem stepProof_kimchiVerify_vesta {kw n : ℕ}
     (havoid : E.σ.Avoids E.lagrangeRelations)
     -- of the proof itself
     (hguard : Guards IpaVesta.curve E.cvk cp pub)
-    (hsg : SgOk E cp pub) :
+    (hsg : SgOk E.σ E.cvk cp pub) :
     kimchiVerify IpaVesta.curve E.σ E.cvk cp pub = true := by
   have hpub := hin.statement
   have hivp := hin.ivpHyps (keyCells := keyCells) (spongeAfterIndex := spongeAfterIndex) hvk
